examples/heapster/linked_list_proofs.v
@@ -1,0 +1,33 @@
+From Coq          Require Import Lists.List.
+From Coq          Require Import String.
+From Coq          Require Import Vectors.Vector.
+From CryptolToCoq Require Import SAWCoreScaffolding.
+From CryptolToCoq Require Import SAWCoreVectorsAsCoqVectors.
+From Records      Require Import Records.
+
+From CryptolToCoq Require Import SAWCorePrelude.
+From CryptolToCoq Require Import CompMExtra.
+
+Load "linked_list.v".
+Import linked_list.
+
+Definition noErrorsSpec {A} : CompM A := existsM (fun a => returnM a).
+
+Import SAWCorePrelude.
+
+
+Lemma no_errors_is_elem : refinesFun is_elem (fun _ _ => noErrorsSpec).
+Proof.
+  unfold is_elem, is_elem__tuple_fun, noErrorsSpec.
+  apply refinesFun_multiFixM_fst. simpl. intros x l.
+  rewrite simpl_letRecM0.
+  apply refinesM_either; intros.
+  - eapply refinesM_existsM_r. reflexivity.
+  - apply refinesM_sigT_rect; intros.
+    apply refinesM_if; intros.
+    + eapply refinesM_existsM_r. reflexivity.
+    + rewrite existsM_bindM.
+      apply refinesM_existsM_l; intros. rewrite returnM_bindM.
+      apply refinesM_sigT_rect; intros.
+      eapply refinesM_existsM_r. reflexivity.
+Qed.
